coq/SemanticsExist.v
@@ -424,3 +424,538 @@ f_equal.
   apply meta_truncate_null.
   }
 Qed.
+
+
+Definition union_action
+  (w : ordinal) (A : wurel w) (B : urelsp_car A -> wurel w)
+  : nat -> relation (wterm w)
+  :=
+  fun i m m' =>
+    (exists r r' (Hr : rel A i r r') n, rel (B (urelspinj A i r r' Hr)) i m n)
+    /\ (exists r r' (Hr : rel A i r r') n, rel (B (urelspinj A i r r' Hr)) i n m')
+    /\ forall j n n' (C : wurel stop),
+         j <= i
+         -> (forall p p' (Hp : rel A j p p'),
+               rel (arrow_urel stop j (extend_urel w stop (B (urelspinj A j p p' Hp))) C) j n n')
+         -> rel C j (app n (map_term (extend w stop) m)) (app n' (map_term (extend w stop) m')).
+
+
+Lemma union_uniform :
+  forall w A (B : urelsp A -n> wurel_ofe w), uniform _ (union_action w A (pi1 B)).
+Proof.
+intros w A B.
+do2 3 split.
+
+(* closed *)
+{
+intros i' m n H.
+destruct H as (Hm & Hn & _).
+split.
+  {
+  destruct Hm as (r & r' & Hr & m' & Hm).
+  refine (urel_closed _#5 Hm andel).
+  }
+
+  {
+  destruct Hn as (r & r' & Hr & n' & Hn).
+  refine (urel_closed _#5 Hn ander).
+  }
+}
+
+(* equiv *)
+{
+intros i' m m' n n' Hclm' Hcln' Hequivm Hequivn H.
+destruct H as ((x & y & Hxy & r & Hmr) & (x' & y' & Hxy' & t & Htn) & Hact).
+do2 2 split; eauto.
+  {
+  exists x, y, Hxy, r.
+  eapply urel_equiv; eauto using equiv_refl.
+  eapply urel_closed_2; eauto.
+  }
+
+  {
+  exists x', y', Hxy', t.
+  eapply urel_equiv; eauto using equiv_refl.
+  eapply urel_closed_1; eauto.
+  }
+intros j p p' C Hj Hp.
+so (urel_closed _#5 (Hp _ _ (urel_downward_leq _#6 Hj Hxy))) as (Hclp & Hclp').
+so (Hact _#4 Hj Hp) as Hrel.
+eapply urel_equiv; eauto.
+  {
+  apply hygiene_auto; cbn; auto using map_hygiene.
+  }
+
+  {
+  apply hygiene_auto; cbn; auto using map_hygiene.
+  }
+
+  {
+  apply equiv_app; auto using equiv_refl, map_equiv.
+  }
+
+  {
+  apply equiv_app; auto using equiv_refl, map_equiv.
+  }
+}
+
+(* zigzag *)
+{
+intros i' m n p q Hmn Hpn Hpq.
+destruct Hmn as (Hm & _ & Hmn).
+destruct Hpn as (_ & _ & Hpn).
+destruct Hpq as (_ & Hq & Hpq).
+do2 2 split; auto.
+intros j r t C Hj Hrt.
+so (Hmn _#4 Hj Hrt) as Hmnrt.
+so (Hpn _#4 Hj Hrt) as Hpnrt.
+so (Hpq _#4 Hj Hrt) as Hpqrt.
+eapply urel_zigzag; eauto.
+}
+
+(* downward *)
+{
+intros i m n H.
+destruct H as (Hm & Hn & Hact).
+do2 2 split; auto.
+  {
+  destruct Hm as (x & y & Hxy & q & H).
+  exists x, y, (urel_downward _#5 Hxy), q.
+  refine (rel_from_dist _#6 _ (urel_downward _#5 H)).
+  apply (pi2 B).
+  apply dist_symm.
+  apply urelspinj_dist.
+  omega.
+  }
+
+  {
+  destruct Hn as (x & y & Hxy & q & H).
+  exists x, y, (urel_downward _#5 Hxy), q.
+  refine (rel_from_dist _#6 _ (urel_downward _#5 H)).
+  apply (pi2 B).
+  apply dist_symm.
+  apply urelspinj_dist.
+  omega.
+  }
+}
+Qed.
+
+
+Definition union_urel w A (B : urelsp A -n> wurel_ofe w) :=
+  mk_urel (union_action w A (pi1 B)) (union_uniform _ _ _).
+
+
+Lemma extend_union_urel :
+  forall v w (h : v <<= w) A B,
+    w <<= stop
+    -> extend_urel v w (union_urel v A B)
+       =
+       union_urel w 
+         (extend_urel v w A)
+         (nearrow_compose2 (deextend_urelsp_ne h A) (extend_urel_ne v w) B).
+Proof.
+intros v w h A B Hwstop.
+apply urel_extensionality.
+fextensionality 3.
+intros i m n.
+cbn.
+pextensionality.
+  {
+  intro H.
+  destruct H as ((x & y & Hxy & r & Hmr) & (x' & y' & Hxy' & t & Htn) & Hact).
+  assert (rel (extend_urel v w A) i (map_term (extend v w) x) (map_term (extend v w) y)) as Hxyw.
+    {
+    cbn.
+    rewrite -> !extend_term_cancel; auto.
+    }
+  assert (rel (extend_urel v w A) i (map_term (extend v w) x') (map_term (extend v w) y')) as Hxyw'.
+    {
+    cbn.
+    rewrite -> !extend_term_cancel; auto.
+    }
+  do2 2 split.
+    {
+    exists (map_term (extend v w) x), (map_term (extend v w) y), Hxyw.
+    exists (map_term (extend v w) r).
+    cbn.
+    rewrite -> extend_term_cancel; auto.
+    rewrite -> deextend_urelsp_urelspinj.
+    force_exact Hmr.
+    f_equal.
+    f_equal.
+    apply urelspinj_equal.
+    rewrite -> extend_term_cancel; auto.
+    }
+
+    {
+    exists (map_term (extend v w) x'), (map_term (extend v w) y'), Hxyw'.
+    exists (map_term (extend v w) t).
+    cbn.
+    rewrite -> extend_term_cancel; auto.
+    rewrite -> deextend_urelsp_urelspinj.
+    force_exact Htn.
+    f_equal.
+    f_equal.
+    apply urelspinj_equal.
+    rewrite -> extend_term_cancel; auto.
+    }
+  intros j p q C Hj Hpq.
+  (* Can't do it directly, because going down to v and back up to w loses information. *)
+  apply (urel_zigzag _#4 (app q (map_term (extend v stop) r)) (app p (map_term (extend v stop) (map_term (extend w v) m)))).
+    {
+    refine (arrow_action_app _#9 (Hpq _ _ (urel_downward_leq _#6 Hj Hxyw)) _).
+    cbn.
+    rewrite -> extend_term_cancel; auto.
+    rewrite -> (extend_term_compose_up v stop w); eauto using le_ord_trans.
+    rewrite -> extend_term_cancel; auto.
+    rewrite -> deextend_urelsp_urelspinj.
+    refine (rel_from_dist _#6 _ (urel_downward_leq _#6 Hj Hmr)).
+    apply (pi2 B).
+    apply dist_symm.
+    apply urelspinj_dist_diff; auto.
+    rewrite -> extend_term_cancel; auto.
+    eapply urel_downward_leq; eauto.
+    }
+
+    {
+    refine (arrow_action_app _#9 (Hpq _ _ (urel_downward_leq _#6 Hj Hxyw)) _).
+    cbn.
+    rewrite -> !(extend_term_compose_up v stop w); eauto using le_ord_trans.
+    rewrite -> !extend_term_cancel; auto.
+    rewrite -> deextend_urelsp_urelspinj.
+    refine (rel_from_dist _#6 _ (urel_downward_leq _#6 Hj Hmr)).
+    apply (pi2 B).
+    apply dist_symm.
+    apply urelspinj_dist_diff; auto.
+    rewrite -> extend_term_cancel; auto.
+    eapply urel_downward_leq; eauto.
+    }
+  apply (urel_zigzag _#4 (app q (map_term (extend v stop) (map_term (extend w v) n))) (app p (map_term (extend v stop) t))).
+    {
+    exploit (Hact j p q C); auto.
+    intros a b Hab.
+    assert (rel (extend_urel v w A) j (map_term (extend v w) a) (map_term (extend v w) b)) as Habw.
+      {
+      cbn.
+      rewrite -> !extend_term_cancel; auto.
+      }
+    so (Hpq _ _ Habw) as H.
+    rewrite <- extend_urel_compose_up in H; auto.
+    rewrite -> deextend_urelsp_urelspinj in H.
+    force_exact H.
+    f_equal.
+    f_equal.
+    f_equal.
+    f_equal.
+    apply urelspinj_equal.
+    rewrite -> extend_term_cancel; auto.
+    }
+
+    {
+    refine (arrow_action_app _#9 (Hpq _ _ (urel_downward_leq _#6 Hj Hxyw')) _).
+    cbn.
+    rewrite -> (extend_term_compose_up v stop w); eauto using le_ord_trans.
+    rewrite -> (extend_term_compose_up v stop w); eauto using le_ord_trans.
+    rewrite -> !extend_term_cancel; auto.
+    rewrite -> deextend_urelsp_urelspinj.
+    refine (rel_from_dist _#6 _ (urel_downward_leq _#6 Hj Htn)).
+    apply (pi2 B).
+    apply dist_symm.
+    apply urelspinj_dist_diff; auto.
+    rewrite -> extend_term_cancel; auto.
+    eapply urel_downward_leq; eauto.
+    }
+
+    {
+    refine (arrow_action_app _#9 (Hpq _ _ (urel_downward_leq _#6 Hj Hxyw')) _).
+    cbn.
+    rewrite -> (extend_term_compose_up v stop w); eauto using le_ord_trans.
+    rewrite -> !extend_term_cancel; auto.
+    rewrite -> deextend_urelsp_urelspinj.
+    refine (rel_from_dist _#6 _ (urel_downward_leq _#6 Hj Htn)).
+    apply (pi2 B).
+    apply dist_symm.
+    apply urelspinj_dist_diff; auto.
+    rewrite -> extend_term_cancel; auto.
+    eapply urel_downward_leq; eauto.
+    }
+  }
+
+  {
+  intro H.
+  destruct H as ((x & y & Hxy & r & Hmr) & (x' & y' & Hxy' & t & Htn) & Hact).
+  do2 2 split.
+    {
+    exists (map_term (extend w v) x), (map_term (extend w v) y), Hxy, (map_term (extend w v) r).
+    rewrite -> deextend_urelsp_urelspinj in Hmr.
+    exact Hmr.
+    }
+
+    {
+    exists (map_term (extend w v) x'), (map_term (extend w v) y'), Hxy', (map_term (extend w v) t).
+    rewrite -> deextend_urelsp_urelspinj in Htn.
+    exact Htn.
+    }
+  intros j p q C Hj Hpq.
+  apply (urel_zigzag _#4 (app q (map_term (extend w stop) r)) (app p (map_term (extend w stop) m))).
+    {
+    refine (arrow_action_app _#9 (Hpq _ _ (urel_downward_leq _#6 Hj Hxy)) _).
+    cbn.
+    rewrite -> extend_term_cancel; eauto using le_ord_trans.
+    rewrite -> extend_term_compose_down; eauto using le_ord_trans.
+    rewrite -> deextend_urelsp_urelspinj in Hmr.
+    cbn in Hmr.
+    refine (rel_from_dist _#6 _ (urel_downward_leq _#6 Hj Hmr)).
+    apply (pi2 B).
+    apply dist_symm.
+    apply urelspinj_dist_diff; auto.
+    eapply urel_downward_leq; eauto.
+    }
+
+    {
+    refine (arrow_action_app _#9 (Hpq _ _ (urel_downward_leq _#6 Hj Hxy)) _).
+    cbn.
+    rewrite -> !extend_term_compose_down; eauto using le_ord_trans.
+    rewrite -> deextend_urelsp_urelspinj in Hmr.
+    cbn in Hmr.
+    refine (rel_from_dist _#6 _ (urel_downward_leq _#6 Hj Hmr)).
+    apply (pi2 B).
+    apply dist_symm.
+    apply urelspinj_dist_diff; auto.
+    eapply urel_downward_leq; eauto.
+    }
+  apply (urel_zigzag _#4 (app q (map_term (extend w stop) n)) (app p (map_term (extend w stop) t))).
+    {
+    exploit (Hact j p q C) as H; auto.
+    intros a b Hab.
+    rewrite <- extend_urel_compose_up; auto.
+    rewrite -> deextend_urelsp_urelspinj.
+    apply Hpq.
+    }
+    
+    {
+    refine (arrow_action_app _#9 (Hpq _ _ (urel_downward_leq _#6 Hj Hxy')) _).
+    cbn.
+    rewrite -> !extend_term_compose_down; eauto using le_ord_trans.
+    rewrite -> deextend_urelsp_urelspinj in Htn.
+    cbn in Htn.
+    refine (rel_from_dist _#6 _ (urel_downward_leq _#6 Hj Htn)).
+    apply (pi2 B).
+    apply dist_symm.
+    apply urelspinj_dist_diff; auto.
+    eapply urel_downward_leq; eauto.
+    }
+
+    {
+    refine (arrow_action_app _#9 (Hpq _ _ (urel_downward_leq _#6 Hj Hxy')) _).
+    cbn.
+    rewrite -> extend_term_cancel; eauto using le_ord_trans.
+    rewrite -> extend_term_compose_down; eauto using le_ord_trans.
+    rewrite -> deextend_urelsp_urelspinj in Htn.
+    cbn in Htn.
+    refine (rel_from_dist _#6 _ (urel_downward_leq _#6 Hj Htn)).
+    apply (pi2 B).
+    apply dist_symm.
+    apply urelspinj_dist_diff; auto.
+    eapply urel_downward_leq; eauto.
+    }
+  }
+Qed.
+
+
+Lemma ceiling_union :
+  forall n w A B,
+    ceiling (S n) (union_urel w A B)
+    =
+    union_urel w
+      (ceiling (S n) A)
+      (nearrow_compose2 (embed_ceiling_ne (S n) A) (ceiling_ne (S n)) B).
+Proof.
+intros n w A B.
+apply urel_extensionality.
+fextensionality 3.
+intros i m p.
+cbn.
+pextensionality.
+  {
+  intros (Hin & Hm & Hn & Hact).
+  do2 2 split; auto.
+    {
+    destruct Hm as (x & y & Hxy & r & Hmr).
+    exists x, y, (conj Hin Hxy), r.
+    split; auto.
+    rewrite -> embed_ceiling_urelspinj.
+    auto.
+    }
+
+    {
+    destruct Hn as (x' & y' & Hxy' & t & Htn).
+    exists x', y', (conj Hin Hxy'), t.
+    split; auto.
+    rewrite -> embed_ceiling_urelspinj.
+    auto.
+    }
+  intros j q r C Hj Hqr.
+  assert (j < S n) as Hjn by omega.
+  exploit (Hact j q r C) as H; auto.
+  intros x y Hxy.
+  so (Hqr x y (conj Hjn Hxy)) as Hqr'.
+  rewrite -> embed_ceiling_urelspinj in Hqr'.
+  rewrite <- ceiling_extend_urel in Hqr'.
+  (* There ought to be a nicer way to do this. *)
+  cbn in Hqr'.
+  decompose Hqr'.
+  intros l l' _ Hclq Hclr Hstepsq Hstepsr Hactqr.
+  exists l, l'.
+  do2 5 split; auto.
+  intros j' t u Hj' Htu.
+  exploit (Hactqr j' t u) as H; auto.
+  split; [omega |].
+  auto.
+  }
+
+  {
+  intros (Hm & Hn & Hact).
+  so Hm as (_ & _ & (Hin & _) & _).
+  split; auto.
+  do2 2 split; auto.
+    {
+    destruct Hm as (x & y & (Hin' & Hxy) & r & Hmr).
+    exists x, y, Hxy, r.
+    destruct Hmr as (_ & Hmr); auto.
+    rewrite -> embed_ceiling_urelspinj in Hmr.
+    auto.
+    }
+
+    {
+    destruct Hn as (x' & y' & (Hin' & Hxy') & t & Htn).
+    exists x', y', Hxy', t.
+    destruct Htn as (_ & Htn); auto.
+    rewrite -> embed_ceiling_urelspinj in Htn.
+    auto.
+    }
+  intros j q r C Hj Hqr.
+  assert (j < S n) as Hjn by omega.
+  exploit (Hact j q r C) as H; auto.
+  intros x y (Hin' & Hxy).
+  so (Hqr x y Hxy) as Hqr'.
+  rewrite -> embed_ceiling_urelspinj.
+  rewrite <- ceiling_extend_urel.
+  cbn in Hqr'.
+  decompose Hqr'.
+  intros l l' _ Hclq Hclr Hstepsq Hstepsr Hactqr.
+  exists l, l'.
+  do2 5 split; auto.
+  intros j' t u Hj' Htu.
+  exploit (Hactqr j' t u) as H; auto.
+  destruct Htu as (_ & Htu).
+  exact Htu.
+  }
+Qed.
+
+
+Definition iuunion (w : ordinal) (A : wiurel w) (B : urelsp (den A) -n> wiurel_ofe w) : wiurel w
+  :=
+  (union_urel w (den A) (nearrow_compose den_ne B),
+   meta_pair (meta_iurel A) 
+     (meta_fn (den A) 
+      (nearrow_compose meta_iurel_ne B))).
+
+
+Lemma extend_iuunion :
+  forall v w (h : v <<= w) A B,
+    w <<= stop
+    -> extend_iurel h (iuunion v A B)
+       =
+       iuunion w (extend_iurel h A)
+         (nearrow_compose
+            (nearrow_compose (extend_iurel_ne h) B)
+            (deextend_urelsp_ne h (den A))).
+Proof.
+intros v w h A B Hwstop.
+unfold iuunion, extend_iurel.
+cbn.
+f_equal.
+  {
+  rewrite -> (extend_union_urel _ _ h); auto.
+  f_equal.
+  apply nearrow_extensionality; auto.
+  }
+unfold meta_iurel.
+cbn.
+rewrite -> !extend_meta_pair.
+rewrite -> extend_meta_urel.
+rewrite -> extend_meta_fn.
+f_equal.
+f_equal.
+f_equal.
+apply exT_extensionality_prop.
+cbn.
+fextensionality 1.
+intro x.
+rewrite -> extend_meta_iurel.
+reflexivity.
+Qed.
+
+
+Lemma iutruncate_iuunion :
+  forall n w A B,
+    iutruncate (S n) (iuunion w A B)
+    =
+    iuunion w 
+      (iutruncate (S n) A)
+      (nearrow_compose
+         (nearrow_compose (iutruncate_ne (S n)) B)
+         (embed_ceiling_ne (S n) (den A))).
+Proof.
+intros n w A B.
+assert (S n > 0) as Hpos by omega.
+unfold iuunion.
+unfold iutruncate.
+unfold den.
+cbn [fst snd].
+f_equal.
+  {
+  rewrite -> ceiling_union.
+  f_equal.
+  apply nearrow_extensionality.
+  auto.
+  }
+
+  {
+  rewrite -> !meta_truncate_pair; auto.
+  f_equal.
+    {
+    apply meta_truncate_iurel; auto.
+    }
+  rewrite -> meta_truncate_fn; auto.
+  f_equal.
+  apply nearrow_extensionality.
+  intro C.
+  cbn -[meta_truncate].
+  apply meta_truncate_iurel; auto.
+  }
+Qed.
+
+
+Lemma iuunion_inj :
+  forall w A A' B B',
+    iuunion w A B = iuunion w A' B'
+    -> eq_dep (wiurel w) (fun r => urelsp (den r) -n> wiurel_ofe w) A B A' B'.
+Proof.
+intros w A A' B B' Heq.
+unfold iuunion in Heq.
+so (f_equal (fun z => snd z) Heq) as Heq'.
+cbn in Heq'.
+so (meta_pair_inj _#5 Heq') as (H3 & H4).
+so (meta_iurel_inj _#3 H3); subst A'.
+so (meta_fn_inj _#5 H4) as H5.
+apply eq_impl_eq_dep_snd.
+clear Heq Heq' H3 H4.
+so (eq_dep_impl_eq_snd _#5 H5) as Heq.
+apply nearrow_extensionality.
+intro x.
+so (f_equal (fun z => pi1 z x) Heq) as Heq'.
+cbn in Heq'.
+eapply meta_iurel_inj; eauto.
+Qed.
