coq/Dynamic.v
@@ -30,6 +30,7 @@ Inductive canon : forall {a}, @operator object a -> Prop :=
 | canon_ctapp          : canon (oper_ctapp _)
 | canon_lam            : canon (oper_lam _)
 | canon_intersect      : canon (oper_intersect _)
+| canon_union          : canon (oper_union _)
 | canon_fut            : canon (oper_fut _)
 | canon_cnext          : canon (oper_cnext _)
 | canon_cprev          : canon (oper_cprev _)
@@ -550,6 +551,12 @@ intros; apply value_i; eauto with dynamic.
 Qed.
 
 
+Lemma value_union : forall {m1 m2}, value (union m1 m2).
+Proof.
+intros; apply value_i; eauto with dynamic.
+Qed.
+
+
 Lemma value_fut : forall {m1}, value (fut m1).
 Proof.
 intros; apply value_i; eauto with dynamic.
@@ -781,6 +788,7 @@ Arguments value_ctlam {object m1 m2 m3}.
 Arguments value_ctapp {object m1 m2}.
 Arguments value_lam {object m1}.
 Arguments value_intersect {object m1 m2}.
+Arguments value_union {object m1 m2}.
 Arguments value_fut {object m1}.
 Arguments value_cnext {object m1}.
 Arguments value_cprev {object m1}.
@@ -821,7 +829,7 @@ Arguments value_extt {object x}.
 Hint Constructors canon : dynamic.
 
 
-Hint Resolve value_univ value_cty value_con value_karrow value_arrow value_pi value_clam value_capp value_ctlam value_ctapp value_lam value_intersect value_fut value_cnext value_cprev value_next value_rec value_equal value_triv value_eqtype value_subtype value_kuniv value_all value_alltp value_exist value_mu value_ispositive value_isnegative value_voidtp value_unittp value_cunit value_booltp value_btrue value_bfalse value_prod value_sigma value_cpair value_cpi1 value_cpi2 value_ppair value_set value_iset value_quotient value_guard value_wt value_ext value_extt : dynamic.
+Hint Resolve value_univ value_cty value_con value_karrow value_arrow value_pi value_clam value_capp value_ctlam value_ctapp value_lam value_intersect value_union value_fut value_cnext value_cprev value_next value_rec value_equal value_triv value_eqtype value_subtype value_kuniv value_all value_alltp value_exist value_mu value_ispositive value_isnegative value_voidtp value_unittp value_cunit value_booltp value_btrue value_bfalse value_prod value_sigma value_cpair value_cpi1 value_cpi2 value_ppair value_set value_iset value_quotient value_guard value_wt value_ext value_extt : dynamic.
 
 
 Hint Resolve var_normal value_normal : dynamic.
