coq/SemanticsSigma.v
@@ -924,3 +924,4 @@ pextensionality.
     }
   }
 Qed.
+
